compiler/backend/proofs/data_to_word_assignProofScript.sml
@@ -803,8 +803,71 @@ Theorem RefByteNoInit_thm:
              state_rel c r1 r2 (s2 with <| locals := LN; clock := new_c |>)
                 r [(RefPtr v,rv)] locs
 Proof
-  (* fs [RefByteNoInit_code_def]
-  \\ fs [do_app_def,do_space_def,EVAL ``op_space_reset (RefByte T)``,do_app_aux_def]
+  (*  \\  \\ fs [word_exp_rw] *)
+  ...
+QED
+*)
+
+
+(* slow refinement *)
+(* 2-length;4-initial value;6-immutable *)
+val RefByteNoInit_code1_def = Define `
+  RefByteNoInit_code1 c =
+      let limit = MIN (2 ** c.len_size) (dimword (:'a) DIV 16) in
+      let h = Op Add [Shift Lsr (Var 2) 2; Const bytes_in_word] in
+      let x = SmallLsr h (dimindex (:'a) - 63) in
+      let y = Shift Lsl h (dimindex (:'a) - shift (:'a) - c.len_size) in
+        list_Seq
+          [BignumHalt 2;
+           Assign 1 x;
+           AllocVar c limit (fromList [();();()]);
+           (* compute length *)
+           Assign 5 (Shift Lsr h (shift (:'a)));
+           Assign 7 (Shift Lsl (Var 5) 2);
+           Assign 9 (Lookup NextFree);
+           (* adjust end of heap *)
+           Assign 1 (Op Add [Var 9;
+                             Shift Lsl (Var 5) (shift (:'a))]);
+           Set NextFree (Op Add [Var 1; Const bytes_in_word]);
+           (* 3 := return value *)
+           Assign 3 (Op Or [Shift Lsl (Op Sub [Var 9; Lookup CurrHeap])
+               (shift_length c − shift (:'a)); Const (1w:'a word)]);
+           (* compute header *)
+           Assign 5 (Op Or [Op Or [y; Const 7w]; Var 6]);
+           (* compute repeated byte *)
+           MakeBytes 4;
+           (* store header *)
+           Store (Var 9) 5;
+           (* write last word of byte array *)
+           Assign 11 (Op And [Shift Lsr (Var 2) 2;
+                              Const (bytes_in_word - 1w)]);
+           Assign 13 (Const 0w);
+           Store (Var 1) 13;
+           WriteLastBytes 1 4 11;
+           Assign 7 (Op Sub [Var 7; Const 4w]);
+           (* write rest of byte array *)
+           Call NONE (SOME Replicate_location)
+             (* ret_loc, addr, v, n, ret_val *)
+             [0;9;4;7;3] NONE]:'a wordLang$prog`;
+
+
+Theorem RefByteNoInit_thm1:
+   state_rel c l1 l2 s (t:('a,'c,'ffi) wordSem$state) [] locs /\
+    get_vars [0;1;2] s.locals = SOME (vals ++ [Number &(if fl then 0 else 4)]) /\
+    t.clock = MustTerminate_limit (:'a) - 1 /\
+    do_app (RefByte fl) vals (dimindex(:'a)) s = Rval (v,s2) ==>
+    ?q r new_c.
+      evaluate (RefByteNoInit_code1 c,t) = (q,r) /\
+      if q = SOME NotEnoughSpace then
+        r.ffi = t.ffi
+      else
+        ?rv. q = SOME (Result (Loc l1 l2) rv) /\
+             state_rel c r1 r2 (s2 with <| locals := LN; clock := new_c |>)
+                r [(v,rv)] locs
+Proof
+  qpat_abbrev_tac`tag = if fl then _ else _`
+  \\ fs [RefByteNoInit_code1_def]
+  \\ fs [do_app_def,do_space_def,EVAL ``op_space_reset (RefByte fl)``,do_app_aux_def]
   \\ Cases_on `vals` \\ fs []
   \\ Cases_on `t'` \\ fs []
   \\ Cases_on `h` \\ fs []
@@ -813,11 +876,15 @@ Proof
   \\ IF_CASES_TAC \\ fs [] \\ rw []
   \\ `good_dimindex (:'a)` by fs [state_rel_def]
   \\ drule0 NONNEG_INT \\ strip_tac \\ rveq \\ fs []
+  \\ rename1`Word v`
   \\ fs[]
-  \\ rename1 `get_vars [0] s.locals = SOME [Number (&i)]`
+  \\ `?(w:8 word). v = w2v w` by (qexists_tac `v2w v`
+          \\ simp[bitstringTheory.w2v_v2w])
+  \\ fs[]
+  \\ rename1 `get_vars [0; 1; 2] s.locals = SOME [Number (&i); Word (w2v w); Number &tag]`
   \\ once_rewrite_tac [list_Seq_def]
   \\ fs [wordSemTheory.evaluate_def,word_exp_rw]
-  \\ rpt_drule0 state_rel_get_vars_IMP \\ strip_tac \\ fs [quantHeuristicsTheory.LIST_LENGTH_1]
+  \\ rpt_drule0 state_rel_get_vars_IMP \\ strip_tac \\ fs [LENGTH_EQ_NUM_compute]
   \\ rveq \\ fs [adjust_var_def,get_vars_SOME_IFF]
   \\ fs [get_vars_SOME_IFF_data]
   \\ drule0 (Q.GEN`a1`(Q.SPEC `0` state_rel_get_var_Number_IMP_alt)) \\ fs []
@@ -830,7 +897,7 @@ Proof
   \\ rpt_drule0 state_rel_get_vars_IMP \\ strip_tac \\ fs [LENGTH_EQ_2]
   \\ rveq \\ fs [adjust_var_def,get_vars_SOME_IFF]
   \\ fs [wordSemTheory.get_var_def]
-  \\ `4 * i < dimword (:'a) /\ w = n2w (4*i)` by
+  \\ `w' = n2w (4 * i) /\ 4 * i < dimword (:'a)` by
    (fs [state_rel_thm]
     \\ full_simp_tac std_ss [GSYM APPEND_ASSOC]
     \\ qpat_x_assum `get_var 0 s.locals = SOME (Number (&i))` assume_tac
@@ -847,6 +914,7 @@ Proof
   \\ IF_CASES_TAC
   THEN1 (fs [shift_def,state_rel_def,
              EVAL ``good_dimindex (:'a)``] \\ rfs []) \\ fs []
+  \\ pop_assum kall_tac
   \\ `n2w (4 * i) ⋙ 2 = (n2w i):'a word` by
    (rewrite_tac [GSYM w2n_11,w2n_lsr]
     \\ fs [ONCE_REWRITE_RULE [MULT_COMM] MULT_DIV]) \\ fs []
@@ -857,15 +925,15 @@ Proof
   \\ `state_rel c l1 l2 s (set_var 1 (Word wA) t) [] locs` by
         fs [wordSemTheory.set_var_def,state_rel_insert_1]
   \\ rpt_drule0 AllocVar_thm
-  \\ `?x. dataSem$cut_env (fromList [()]) s.locals = SOME x` by
-    (fs [EVAL ``sptree$fromList [()]``,cut_env_def,domain_lookup,
+   \\ `?x. dataSem$cut_env (fromList [();();()]) s.locals = SOME x` by
+    (fs [EVAL ``sptree$fromList [(); (); ()]``,cut_env_def,domain_lookup,
          get_var_def,get_vars_SOME_IFF_data])
   \\ disch_then drule0
   \\ fs [wordSemTheory.get_vars_def,wordSemTheory.get_var_def]
   \\ qabbrev_tac `limit = MIN (2 ** c.len_size) (dimword (:α) DIV 16)`
   \\ fs [get_var_set_var_thm]
   \\ Cases_on `evaluate
-       (AllocVar c limit (fromList [()]),set_var 1 (Word wA) t)` \\ fs []
+       (AllocVar c limit (fromList [(); (); ()]),set_var 1 (Word wA) t)` \\ fs []
   \\ disch_then drule0
   \\ impl_tac THEN1 (unabbrev_all_tac \\ fs []
                      \\ fs [state_rel_def,EVAL ``good_dimindex (:'a)``,dimword_def])
@@ -881,35 +949,532 @@ Proof
   \\ fs [] \\ once_rewrite_tac [list_Seq_def]
   \\ once_rewrite_tac [wordSemTheory.evaluate_def]
   \\ simp [Once wordSemTheory.evaluate_def]
-  \\  \\ fs [word_exp_rw] *)
-  ...
+  \\ fs [word_exp_rw]
+  \\ `lookup 2 r.locals = SOME (Word (n2w (4 * i)))` by
+   (qabbrev_tac `s9 = s with <|locals := x; space := w2n wA DIV 4 + 1|>`
+    \\ fs [state_rel_def,get_vars_SOME_IFF_data]
+    \\ full_simp_tac std_ss [GSYM APPEND_ASSOC,get_var_def]
+    \\ rpt_drule0 word_ml_inv_get_var_IMP
+    \\ fs [get_var_def,wordSemTheory.get_var_def,adjust_var_def]
+    \\ `lookup 0 s9.locals = SOME (Number (&i))` by
+     (unabbrev_all_tac \\ fs [cut_env_def] \\ rveq
+      \\ fs [lookup_inter_alt] \\ EVAL_TAC)
+    \\ rpt (disch_then drule0) \\ fs []
+    \\ `IS_SOME (lookup 0 s9.locals)` by fs []
+    \\ res_tac \\ Cases_on `lookup 2 r.locals` \\ fs []
+    \\ fs [word_ml_inv_def] \\ rw []
+    \\ fs [abs_ml_inv_def,bc_stack_ref_inv_def,v_inv_def] \\ rfs []
+    \\ rw [] \\ fs [word_addr_def,Smallnum_def]
+    \\ fs [small_int_def,X_LT_DIV]
+    \\ match_mp_tac minus_2_word_and_id
+    \\ fs [word_index,word_mul_n2w,bitTheory.BIT0_ODD,ODD_MULT])
+  \\ `~(2 ≥ dimindex (:α))` by (fs [good_dimindex_def])
+  \\ `shift (:α) ≠ 0 /\ ~(shift (:α) ≥ dimindex (:α))` by
+        (rw [shift_def] \\ fs [good_dimindex_def])
+  \\ simp []
+  \\ simp [Once wordSemTheory.evaluate_def]
+  \\ simp [Once wordSemTheory.evaluate_def]
+  \\ simp [Once wordSemTheory.evaluate_def]
+  \\ simp [Once wordSemTheory.evaluate_def]
+  \\ fs [word_exp_rw]
+  \\ `(?free. FLOOKUP r.store NextFree = SOME (Word free)) /\
+      (?eoh1. FLOOKUP r.store EndOfHeap = SOME (Word eoh1)) /\
+      (?cur1. FLOOKUP r.store CurrHeap = SOME (Word cur1))` by
+        (fs [state_rel_thm,memory_rel_def,heap_in_memory_store_def])
+  \\ fs []
+  \\ `lookup 4 r.locals = SOME (Word (w2w w << (dimindex(:'a) - 8)))`
+  by (qabbrev_tac `s9 = s with <|locals := x; space := w2n wA DIV 4 + 1|>`
+    \\ fs [state_rel_def,get_vars_SOME_IFF_data]
+    \\ full_simp_tac std_ss [GSYM APPEND_ASSOC,get_var_def]
+    \\ rpt_drule0 word_ml_inv_get_var_IMP
+    \\ fs [get_var_def,wordSemTheory.get_var_def,adjust_var_def]
+    \\ `lookup 1 s9.locals = SOME (Word (w2v w))` by
+     (unabbrev_all_tac \\ fs [cut_env_def] \\ rveq
+      \\ fs [lookup_inter_alt] \\ EVAL_TAC)
+    \\ rpt (disch_then drule0) \\ fs[]
+    \\ `IS_SOME (lookup 1 s9.locals)` by fs []
+    \\ res_tac \\ Cases_on `lookup 4 r.locals` \\ fs []
+    \\ fs [word_ml_inv_def] \\ rw []
+    \\ fs [abs_ml_inv_def,bc_stack_ref_inv_def,v_inv_def] \\ rfs []
+    \\ rw []
+    \\ `8 <= dimindex(:'a)-2` by fs[good_dimindex_def] \\ fs[]
+    \\ fs[word_addr_def]
+    \\ `!(w:word8). v2w (w2v w) = (w2w w):('a word)` by (
+        rw[] \\ simp[v2w_def,w2w_def]
+        \\ simp[n2w_def]
+        \\ simp[CART_EQ]
+        \\ rw[BIT_w2n,FCP_BETA]
+        \\ fs[testbit]
+        \\ rename1`BIT ii (w2n ww)`
+        \\ ASSUME_TAC (Q.SPECL[`ii`,`ww`](INST_TYPE[alpha|->``:8``]BIT_w2n))
+        \\ fs[]
+        \\ Cases_on`ii<8` \\ fs[EL_w2v]
+        \\ ASSUME_TAC(Q.ISPEC`ww:word8`w2n_lt)
+        \\ `w2n ww < 2**ii` by (match_mp_tac LESS_LESS_EQ_TRANS
+           \\ qexists_tac`2**8` \\ fs[dimword_def]
+        )
+        \\ `w2n ww DIV 2**ii = 0` by (match_mp_tac DIV_UNIQUE \\ simp[])
+        \\ fs[]
+        \\ simp[bitTheory.BITS_THM,bitTheory.BIT_def])
+   \\ fs[]
+   \\ simp[word_and_def,word_lsl_def]
+   \\ simp[fcpTheory.CART_EQ,fcpTheory.FCP_BETA]
+   \\ rw[]
+   \\ rename1`_ <= j +8`
+   \\ Cases_on`dimindex(:'a) <= j+8` \\ fs[]
+   \\ simp[word_2comp_def]
+   \\ `2 MOD dimword(:'a)=2` by (fs[dimword_def,good_dimindex_def])
+   \\ fs[]
+   \\ Q.MATCH_ABBREV_TAC`_ /\ X <=> X`
+   \\ Cases_on`X` \\ fs[]
+   \\ simp[n2w_def]
+   \\ simp[fcpTheory.FCP_BETA]
+   \\ simp[bitTheory.BITS_THM,bitTheory.BIT_def]
+   \\ match_mp_tac MOD_UNIQUE
+   \\ simp[]
+   \\ simp[dimword_def]
+   \\ ASSUME_TAC(Q.SPECL[`2`,`dimindex(:'a)`,`2`,`j`]EXP_SUB_DIV)
+   \\ pop_assum mp_tac
+   \\ Cases_on `j` \\ fs[]
+   \\ rw[]
+   \\ Q.PAT_ABBREV_TAC`X = (2:num) ** _`
+   \\ qexists_tac`X DIV 2 - 1`
+   \\ UNABBREV_ALL_TAC \\ fs[]
+   \\ Cases_on`dimindex(:'a) - SUC n` >- fs[]
+   \\ `2 ** SUC n' DIV 2 = 2 ** n'` by (match_mp_tac DIV_UNIQUE \\
+   qexists_tac`0` \\ simp[EXP])
+   \\ fs[]
+   \\ simp[LEFT_SUB_DISTRIB]
+   \\ simp[EXP]
+   \\ Cases_on`2 * 2 ** n'` \\ fs[]
+   \\ Cases_on`n''` \\ fs[]
+    )
+    \\ fs[]
+  \\ `lookup 6 r.locals = SOME (Word (n2w (4 * tag)))` by
+   (qabbrev_tac `s9 = s with <|locals := x; space := w2n wA DIV 4 + 1|>`
+    \\ fs [state_rel_def,get_vars_SOME_IFF_data]
+    \\ full_simp_tac std_ss [GSYM APPEND_ASSOC,get_var_def]
+    \\ rpt_drule0 word_ml_inv_get_var_IMP
+    \\ fs [get_var_def,wordSemTheory.get_var_def,adjust_var_def]
+    \\ `lookup 2 s9.locals = SOME (Number &tag)` by
+     (unabbrev_all_tac \\ fs [cut_env_def] \\ rveq
+      \\ fs [lookup_inter_alt] \\ EVAL_TAC)
+    \\ rpt (disch_then drule0) \\ fs []
+    \\ `IS_SOME (lookup 2 s9.locals)` by fs []
+    \\ res_tac \\ Cases_on `lookup 6 r.locals` \\ fs []
+    \\ fs [word_ml_inv_def] \\ rw []
+    \\ fs [abs_ml_inv_def,bc_stack_ref_inv_def,v_inv_def] \\ rfs []
+    \\ `small_int (:'a) (&tag)`
+    by (
+      rw[small_int_def,Abbr`tag`]
+      \\ fs[labPropsTheory.good_dimindex_def,dimword_def] )
+    \\ fs[word_addr_def,Smallnum_def]
+    \\ match_mp_tac minus_2_word_and_id
+    \\ simp[word_index,bitTheory.BIT0_ODD,ODD_MULT])
+  \\ fs[wordSemTheory.set_var_def,lookup_insert]
+  \\ fs [] \\ once_rewrite_tac [list_Seq_def]
+  \\ fs [wordSemTheory.evaluate_def,word_exp_rw,wordSemTheory.set_var_def]
+  \\ once_rewrite_tac [list_Seq_def]
+  \\ fs [wordSemTheory.evaluate_def,word_exp_rw,wordSemTheory.set_var_def,
+         wordSemTheory.set_store_def]
+  \\ once_rewrite_tac [list_Seq_def]
+  \\ fs [wordSemTheory.evaluate_def,word_exp_rw,wordSemTheory.set_var_def,
+         wordSemTheory.set_store_def,FLOOKUP_UPDATE]
+  \\ IF_CASES_TAC
+  THEN1 (fs [shift_def,shift_length_def,state_rel_def,
+                 EVAL ``good_dimindex (:'a)``] \\ fs [])
+  \\ pop_assum kall_tac \\ fs []
+  \\ qabbrev_tac `var5 = (bytes_in_word + n2w i:'a word) ⋙ shift (:α)`
+  \\ once_rewrite_tac [list_Seq_def]
+  \\ fs [wordSemTheory.evaluate_def,word_exp_rw,wordSemTheory.set_var_def,
+         wordSemTheory.set_store_def]
+  \\ once_rewrite_tac [list_Seq_def]
+  \\ fs [wordSemTheory.evaluate_def,word_exp_rw,wordSemTheory.set_var_def,
+         wordSemTheory.set_store_def]
+  \\ fs [evaluate_MakeBytes,word_exp_rw,wordSemTheory.set_var_def,
+         lookup_insert,wordSemTheory.get_var_def,w2w_shift_shift]
+  \\ qpat_assum `state_rel c l1 l2 _ _ _ _` mp_tac
+  \\ simp_tac std_ss [Once state_rel_thm] \\ strip_tac \\ fs []
+  \\ `w2n wA DIV 4 = byte_len (:'a) i` by
+   (unabbrev_all_tac \\ fs [byte_len_def,bytes_in_word_def,w2n_lsr,
+      labPropsTheory.good_dimindex_def,word_add_n2w,dimword_def] \\ rfs []
+    \\ fs [GSYM word_add_n2w] \\ fs [word_add_n2w,dimword_def]
+    \\ fs [ADD_DIV_EQ,DIV_DIV_DIV_MULT])
+  \\ fs [wordSemTheory.set_var_def,lookup_insert]
+  \\ rpt_drule0 memory_rel_RefByte_alt
+  \\ disch_then (qspecl_then [`w`,`i`,`fl`] mp_tac) \\ fs []
+  \\ impl_tac THEN1
+   (unabbrev_all_tac \\ fs []
+    \\ fs [labPropsTheory.good_dimindex_def,dimword_def] \\ rfs [])
+   \\ strip_tac \\ fs [FLOOKUP_DEF] \\ rveq \\ clean_tac
+  \\ `var5 = n2w (byte_len (:α) i)` by
+   (unabbrev_all_tac
+    \\ rewrite_tac [GSYM w2n_11,w2n_lsr,byte_len_def]
+    \\ fs [bytes_in_word_def,shift_def,labPropsTheory.good_dimindex_def]
+    \\ fs [word_add_n2w,ADD_DIV_EQ]
+    THEN1
+     (sg `i + 4 < dimword (:'a)`
+      \\ sg `i + 4 DIV 4 < dimword (:'a)` \\ fs []
+      \\ rfs [dimword_def] \\ fs [DIV_LT_X])
+    THEN1
+     (sg `i + 8 < dimword (:'a)`
+      \\ sg `i + 8 DIV 8 < dimword (:'a)` \\ fs []
+      \\ rfs [dimword_def] \\ fs [DIV_LT_X]))
+  \\ fs [] \\ rveq
+  \\ once_rewrite_tac [list_Seq_def]
+  \\ fs [wordSemTheory.evaluate_def,word_exp_rw,wordSemTheory.set_var_def,
+         wordSemTheory.set_store_def,wordSemTheory.get_var_def,lookup_insert,
+         wordSemTheory.mem_store_def,store_list_def]
+  \\ once_rewrite_tac [list_Seq_def]
+  \\ simp[Once wordSemTheory.evaluate_def,
+          wordSemTheory.get_var_def,lookup_insert,
+          wordSemTheory.get_var_imm_def,
+          asmTheory.word_cmp_def]
+  \\ rfs [shift_lsl,GSYM word_add_n2w,WORD_LEFT_ADD_DISTRIB]
+  \\ qpat_abbrev_tac `ppp = Word (_ || _:'a word)`
+  \\ `ppp = Word (make_byte_header c fl i)` by
+   (unabbrev_all_tac \\ fs [make_byte_header_def,bytes_in_word_def]
+    \\ Cases_on`fl`
+    \\ fs [labPropsTheory.good_dimindex_def,GSYM word_add_n2w,WORD_MUL_LSL]
+    \\ fs [word_mul_n2w,word_add_n2w,shift_def,RIGHT_ADD_DISTRIB])
+  \\ rveq \\ pop_assum kall_tac
+   \\ fs [wordSemTheory.evaluate_def,word_exp_rw,
+         wordSemTheory.get_var_def,lookup_insert,
+         wordSemTheory.mem_store_def,store_list_def]
+  \\ once_rewrite_tac[list_Seq_def]
+  \\ simp[wordSemTheory.evaluate_def,word_exp_rw]
+  \\ simp[wordSemTheory.set_var_def]
+  \\ once_rewrite_tac[list_Seq_def]
+  \\ simp[wordSemTheory.evaluate_def,word_exp_rw,
+          asmTheory.word_cmp_def,wordSemTheory.get_var_def]
+  \\ `(bytes_in_word:'a word) + -1w = n2w (2 ** shift(:'a) - 1)`
+  by ( fs[bytes_in_word_def,labPropsTheory.good_dimindex_def,shift_def] )
+  \\ simp[WORD_AND_EXP_SUB1]
+  \\ `i MOD 2 ** (shift(:'a)) < dimword(:'a)`
+  by (
+    match_mp_tac LESS_LESS_EQ_TRANS
+    \\ qexists_tac`2 ** shift(:'a)`
+    \\ simp[]
+    \\ fs[labPropsTheory.good_dimindex_def,dimword_def,shift_def] )
+  \\ simp[]
+  \\ `2 ** shift(:'a) = dimindex(:'a) DIV 8`
+    by ( fs[labPropsTheory.good_dimindex_def,dimword_def,shift_def] )
+  \\ simp[]
+  \\ simp[(* CONJUNCT2 (CONJUNCT2 list_Seq_def), *)
+          wordSemTheory.evaluate_def,word_exp_rw,
+          wordSemTheory.set_var_def,
+          wordSemTheory.mem_store_def,
+          wordSemTheory.get_var_def,lookup_insert]
+  \\ reverse IF_CASES_TAC
+  >- (
+    `F` suffices_by rw[]
+    \\ pop_assum mp_tac \\ simp []
+    \\ imp_res_tac store_list_domain
+    \\ fs[LENGTH_REPLICATE]
+    \\ first_x_assum(qspec_then`byte_len(:'a) i-1`mp_tac)
+    \\ simp[]
+    \\ fs[WORD_MUL_LSL,word_mul_n2w]
+    \\ Cases_on`byte_len(:'a) i = 0` \\ fs[]
+    \\ Cases_on`byte_len(:'a) i` \\ fs[ADD1,GSYM word_add_n2w]
+    \\ simp[WORD_MULT_CLAUSES,WORD_LEFT_ADD_DISTRIB])
+  \\ fs[]
+  \\ simp[CONJUNCT2 (CONJUNCT2 list_Seq_def),
+          wordSemTheory.evaluate_def,word_exp_rw,
+          wordSemTheory.set_var_def,
+          wordSemTheory.mem_store_def,
+          wordSemTheory.get_var_def,lookup_insert]
+  \\ pairarg_tac \\ fs[]
+  \\ pairarg_tac \\ fs[]
+  \\ pop_assum mp_tac
+  \\ pop_assum mp_tac
+   \\ assume_tac(GEN_ALL evaluate_WriteLastBytes)
+  \\ SEP_I_TAC "evaluate"
+  \\ pop_assum mp_tac
+  \\ simp[wordSemTheory.get_vars_def,wordSemTheory.get_var_def,lookup_insert,APPLY_UPDATE_THM]
+  \\ impl_tac
+  >- (conj_tac >- fs[good_dimindex_def]
+     \\ fs[memory_rel_def,heap_in_memory_store_def,FLOOKUP_UPDATE]
+     \\ fs[FLOOKUP_DEF]
+     \\ qpat_x_assum `free' + bytes_in_word + _ = _` mp_tac
+     \\ simp_tac std_ss [WORD_ADD_EQ_SUB]
+     \\ simp[aligned_add_sub] \\ rpt strip_tac \\ rveq
+     \\ fs [byte_aligned_def]
+     \\ rewrite_tac [GSYM WORD_ADD_ASSOC]
+     \\ (alignmentTheory.aligned_add_sub_cor
+           |> SPEC_ALL |> UNDISCH_ALL |> CONJUNCT1 |> DISCH_ALL |> match_mp_tac)
+     \\ fs []
+     \\ (alignmentTheory.aligned_add_sub_cor
+           |> SPEC_ALL |> UNDISCH_ALL |> CONJUNCT1 |> DISCH_ALL |> match_mp_tac)
+     \\ fs [GSYM byte_aligned_def]
+     \\ fs [byte_aligned_bytes_in_word])
+   \\ simp[] \\ disch_then kall_tac
+  \\ strip_tac \\ fs[] \\ clean_tac \\ fs[]
+  \\ fs [lookup_insert]
+  \\ strip_tac \\ rveq \\ fs []
+  \\ pop_assum mp_tac \\ simp[list_Seq_def]
+  \\ strip_tac \\ clean_tac \\ fs[]
+  \\ `lookup Replicate_location r.code = SOME (5,Replicate_code)` by
+         (imp_res_tac lookup_RefByte_location) \\ rfs []
+  \\ qmatch_asmsub_abbrev_tac`LUPDATE lw (len-1) ls`
+  \\ qmatch_assum_abbrev_tac`Abbrev(ls = REPLICATE len rw)`
+  \\ `0 < len` by ( Cases_on`len` \\ fs[byte_len_def,markerTheory.Abbrev_def] )
+  \\ `ls = REPLICATE (len-1) rw ++ [rw] ++ []`
+   by (
+    simp[Abbr`ls`,LIST_EQ_REWRITE,EL_REPLICATE,LENGTH_REPLICATE]
+    \\ qx_gen_tac`z` \\ strip_tac
+    \\ Cases_on`z = len-1` \\ simp[EL_APPEND1,EL_APPEND2,EL_REPLICATE,LENGTH_REPLICATE] )
+  \\ `LUPDATE lw (len-1) ls = REPLICATE (len-1) rw ++ [lw] ++ []` by metis_tac[lupdate_append2,LENGTH_REPLICATE]
+  \\ pop_assum SUBST_ALL_TAC
+  \\ pop_assum kall_tac \\ fs[]
+  \\ imp_res_tac store_list_append_imp
+  \\ assume_tac (GEN_ALL Replicate_code_thm)
+  \\ SEP_I_TAC "evaluate"
+  \\ pop_assum mp_tac \\ fs[wordSemTheory.get_var_def,lookup_insert]
+  \\ simp[UPDATE_EQ]
+  \\ qmatch_goalsub_abbrev_tac`(a' =+ v)`
+  \\ qhdtm_x_assum`store_list`mp_tac
+  \\ drule0 (Q.GEN`a'`store_list_update_m_outside)
+  \\ disch_then(qspec_then`a'`mp_tac)
+  \\ impl_tac
+   >- (
+    simp[Abbr`a'`,LENGTH_REPLICATE]
+    \\ rewrite_tac[GSYM WORD_ADD_ASSOC]
+    \\ simp[WORD_EQ_ADD_LCANCEL]
+    \\ CONV_TAC(PATH_CONV"brrlrr"(REWR_CONV WORD_MULT_COMM))
+    \\ rewrite_tac[GSYM WORD_MULT_ASSOC]
+    \\ `len < dimword (:α) DIV 16` by
+          (unabbrev_all_tac \\ fs [])
+    \\ qpat_x_assum `good_dimindex (:'a)` mp_tac
+    \\ pop_assum mp_tac
+    \\ rpt (pop_assum kall_tac)
+    \\ fs [good_dimindex_def] \\ rw [] \\ fs [bytes_in_word_def]
+    \\ fs [word_add_n2w,word_mul_n2w,dimword_def])
+  \\ ntac 2 strip_tac \\ rfs[]
+  \\ `n2w len << 2 + -4w = n2w (4 * (len - 1))` by (
+      simp[word_lsl_n2w]
+      \\ REWRITE_TAC[word_2comp_n2w]
+      \\ `4 MOD dimword(:'a) = 4` by fs[good_dimindex_def,dimword_def]
+      \\ fs[]
+      \\ simp[word_add_n2w]
+      \\ `4 * len + dimword (:α) - 4 = (4*len - 4) + dimword(:'a)` by (
+         ONCE_REWRITE_TAC[ADD_COMM]
+         \\ match_mp_tac LESS_EQ_ADD_SUB
+         \\ simp[]
+      )
+      \\ pop_assum(fn a=> SUBST_TAC[a])
+      \\ ONCE_REWRITE_TAC[ADD_COMM]
+      \\ simp[ADD_MODULUS]
+      \\ simp[LEFT_SUB_DISTRIB]
+  )
+  \\ pop_assum SUBST_ALL_TAC
+  \\ disch_then (mp_tac o Q.SPEC`len - 1`)
+  \\ `Word (word_of_byte2 (w2w w << (dimindex(:'a)-8))) = rw` by (
+     simp[Abbr`rw`]
+     \\ simp[word_of_byte2_def,word_of_byte_def]
+     \\ `(w2w w) << 24 >>> 24 = w2w w` by (
+        match_mp_tac lsl_lsr
+        \\ match_mp_tac LESS_LESS_EQ_TRANS
+        \\ qexists_tac`2 ** 8 * 2 ** 24`
+        \\ simp[]
+        \\ reverse conj_tac
+        >-(fs[good_dimindex_def,dimword_def])
+        \\ simp[w2n_w2w]
+        \\ `8<=dimindex(:'a)` by fs[good_dimindex_def]
+        \\ fs[]
+        \\ `256 = dimword(:8)` by simp[dimword_def]
+        \\ pop_assum SUBST_ALL_TAC
+        \\ simp[w2n_lt]
+     )
+     \\ simp[]
+     \\ TOP_CASE_TAC \\ simp[]
+     >-(MK_COMB_TAC \\ simp[]
+        \\ GEN_REWRITE_TAC(ONCE_DEPTH_CONV o LAND_CONV)empty_rewrites[WORD_OR_COMM]
+        \\ GEN_REWRITE_TAC(ONCE_DEPTH_CONV o RAND_CONV)empty_rewrites[GSYM WORD_OR_ASSOC]
+        \\ MK_COMB_TAC \\ simp[]
+        \\ MK_COMB_TAC \\ simp[]
+        \\ `(w2w (w:word8):'a word) ≪ 24 ⋙ 8 = w2w w << 16` by (
+           simp[word_lsl_def,fcpTheory.CART_EQ]
+           \\ rw[fcpTheory.FCP_BETA]
+           \\ rename1`j<32`
+           \\ reverse(Cases_on`16<=j` \\ simp[])
+           >-(
+              simp[word_lsr_def,fcpTheory.FCP_BETA]
+           )
+           \\ simp[word_lsr_def,fcpTheory.FCP_BETA]
+           \\ reverse(Cases_on`j+8 < 32`) \\ fs[]
+           >-simp[w2w]
+           \\ simp[fcpTheory.FCP_BETA]
+        )
+        \\ simp[]
+        \\ GEN_REWRITE_TAC(ONCE_DEPTH_CONV o LAND_CONV)empty_rewrites[WORD_OR_COMM]
+        \\ MK_COMB_TAC \\ simp[]
+        \\ MK_COMB_TAC \\ simp[]
+        \\ simp[word_lsl_def,fcpTheory.CART_EQ]
+        \\ rw[fcpTheory.FCP_BETA]
+        \\ rename1`j<32`
+        \\ reverse(Cases_on`8<=j` \\ simp[])
+        >-(
+           simp[word_lsr_def,fcpTheory.FCP_BETA]
+        )
+        \\ simp[word_lsr_def,fcpTheory.FCP_BETA]
+        \\ reverse(Cases_on`j+16 < 32`) \\ fs[]
+        >-simp[w2w]
+        \\ simp[fcpTheory.FCP_BETA])
+   \\ `dimindex(:'a) = 64` by fs[good_dimindex_def]
+   \\ fs[]
+   \\ `!x. x<= 56 ==> w2w (w:word8) << 56 >>> x = w2w w << (56 - x)` by(
+      rw[]
+      \\ simp[word_lsr_def,fcpTheory.FCP_BETA,fcpTheory.CART_EQ]
+      \\ rw[]
+      \\ rename1`j+xx<64`
+      \\ reverse(Cases_on`j+xx<64` \\ fs[])
+      >- (Q.MATCH_GOALSUB_ABBREV_TAC`X ' j`
+          \\ `X ' j <=> word_bit j X` by (simp[word_bit])
+          \\ simp[]
+          \\ simp[Abbr`X`]
+          \\ simp[word_bit_lsl]
+          \\ `dimindex(:8) <= dimindex(:'a)` by fs[]
+          \\ simp[word_bit_w2w]
+      )
+      \\ Q.MATCH_GOALSUB_ABBREV_TAC`X ' j`
+      \\ `X ' j <=> word_bit j X` by (simp[word_bit])
+      \\ simp[]
+      \\ simp[Abbr`X`]
+      \\ simp[word_bit_lsl]
+      \\ Q.MATCH_GOALSUB_ABBREV_TAC`X ' (j+xx)`
+      \\ `X ' (j+xx) <=> word_bit (j+xx) X` by (
+         simp[word_bit]
+      )
+      \\ simp[]
+      \\ simp[Abbr`X`]
+      \\ simp[word_bit_lsl]
+   )
+   \\ fs[])
+  \\ fs[]
+  \\ impl_tac
+  >-(UNABBREV_ALL_TAC \\ fs[byte_len_def]
+     \\ `s.clock <> 0` by (
+        fs[state_rel_thm]
+     )
+     \\ fs[]
+     \\ fs[good_dimindex_def] \\ fs[]
+     \\ (Q.UNDISCH_TAC`small_int (:α) (&i)`
+        \\ simp[small_int_def]
+        \\ strip_tac
+        \\ simp[DIV_TIMES]
+        \\ Q.MATCH_ASMSUB_ABBREV_TAC`state_rel c l1 l2 s X`
+        \\ Q.UNDISCH_TAC`state_rel c l1 l2 s X [] locs`
+        \\ simp[state_rel_thm]
+        \\ UNABBREV_ALL_TAC \\ simp[]
+        \\ strip_tac
+        \\ Q.UNDISCH_TAC`MustTerminate_limit (:α) - 1 = s.clock`
+        \\ Q.UNDISCH_TAC`i < dimword(:'a) DIV 8`
+        \\ simp[wordSemTheory.MustTerminate_limit_def]
+        \\ strip_tac
+        \\ disch_then(SUBST_ALL_TAC o GSYM)
+        \\ simp[DIV_LT_X]
+     )
+     \\ fs[X_LT_DIV]
+  )
+  \\ strip_tac \\ fs[]
+  \\ simp [state_rel_thm]
+  \\ fs []
+  \\ fs [lookup_def]
+  \\ qhdtm_x_assum `memory_rel` mp_tac
+  \\ fs [EVAL ``join_env LN []``,code_oracle_rel_def,FLOOKUP_UPDATE]
+  \\ fs[store_list_def]
+  \\ fs[Abbr`a'`,Abbr`v`,LENGTH_REPLICATE]
+  \\ clean_tac
+  \\ fs[make_ptr_def,WORD_MUL_LSL]
+  \\ qmatch_abbrev_tac`P xx yy zz ⇒ P x' yy z'`
+  \\ `xx = x'`
+  by (
+    simp[Abbr`xx`,Abbr`x'`,FUN_EQ_THM,APPLY_UPDATE_THM,Abbr`lw`]
+    \\ simp[n2w_sub,WORD_LEFT_ADD_DISTRIB] \\ rw[]
+    \\ simp[w2w_word_of_byte_w2w]
+    \\ ntac 2 (MK_COMB_TAC \\ simp[])
+    \\ MK_COMB_TAC \\ simp[]
+    \\ MK_COMB_TAC \\ simp[]
+    \\ REWRITE_TAC[word_of_byte2_def]
+    \\ SIMP_TAC std_ss []
+    \\ REWRITE_TAC[fcpTheory.CART_EQ]
+    \\ ntac 2 strip_tac
+    \\ ASM_SIMP_TAC std_ss [w2w]
+    \\ rename1`j < dimindex(:'a)`
+    \\ `j<dimindex(:'a)` by fs[good_dimindex_def]
+    \\ ASM_SIMP_TAC std_ss[]
+    \\ REWRITE_TAC[LET_THM]
+    \\ simp[n2w_2exp_mult]
+    \\ TOP_CASE_TAC
+    \\ fs[good_dimindex_def]
+    \\ (simp[word_or_def,fcpTheory.FCP_BETA]
+       \\ simp[word_bit]
+       \\ simp[word_bit_lsl,word_bit_lsr,word_bit_w2w]
+       \\ fs[]
+    ))
+  \\ rveq \\ qunabbrev_tac `P`
+  \\ match_mp_tac memory_rel_rearrange
+  \\ unabbrev_all_tac \\ rpt (pop_assum kall_tac)
+  \\ fs[FAPPLY_FUPDATE_THM]
+  \\ rw [] \\ fs []
 QED
-*)
 
-Theorem RefByteNoInit_thm:
+(* version with implicit T in immutable *)
+val RefByteNoInit_code2_def = Define `
+  RefByteNoInit_code2 c =
+      let limit = MIN (2 ** c.len_size) (dimword (:'a) DIV 16) in
+      let h = Op Add [Shift Lsr (Var 2) 2; Const bytes_in_word] in
+      let x = SmallLsr h (dimindex (:'a) - 63) in
+      let y = Shift Lsl h (dimindex (:'a) - shift (:'a) - c.len_size) in
+        list_Seq
+          [BignumHalt 2;
+           Assign 1 x;
+           AllocVar c limit (fromList [();()]);
+           (* compute length *)
+           Assign 5 (Shift Lsr h (shift (:'a)));
+           Assign 7 (Shift Lsl (Var 5) 2);
+           Assign 9 (Lookup NextFree);
+           (* adjust end of heap *)
+           Assign 1 (Op Add [Var 9;
+                             Shift Lsl (Var 5) (shift (:'a))]);
+           Set NextFree (Op Add [Var 1; Const bytes_in_word]);
+           (* 3 := return value *)
+           Assign 3 (Op Or [Shift Lsl (Op Sub [Var 9; Lookup CurrHeap])
+               (shift_length c − shift (:'a)); Const (1w:'a word)]);
+           (* compute header *)
+           Assign 5 (Op Or [y; Const 7w]);
+           (* compute repeated byte *)
+           MakeBytes 4;
+           (* store header *)
+           Store (Var 9) 5;
+           (* write last word of byte array *)
+           Assign 11 (Op And [Shift Lsr (Var 2) 2;
+                              Const (bytes_in_word - 1w)]);
+           Assign 13 (Const 0w);
+           Store (Var 1) 13;
+           WriteLastBytes 1 4 11;
+           Assign 7 (Op Sub [Var 7; Const 4w]);
+           (* write rest of byte array *)
+           Call NONE (SOME Replicate_location)
+             (* ret_loc, addr, v, n, ret_val *)
+             [0;9;4;7;3] NONE]:'a wordLang$prog`;
+
+
+Theorem RefByteNoInit_thm2:
    state_rel c l1 l2 s (t:('a,'c,'ffi) wordSem$state) [] locs /\
     get_vars [0;1] s.locals = SOME vals /\
     t.clock = MustTerminate_limit (:'a) - 1 /\
-    EL 0 vals = Number arrl /\
     do_app (RefByte T) vals (dimindex(:'a)) s = Rval (v,s2) ==>
-    ?q r new_c anyptr arr.
-     evaluate (RefByteNoInit_code c,t) = (q,r) /\
+    ?q r new_c.
+      evaluate (RefByteNoInit_code2 c,t) = (q,r) /\
       if q = SOME NotEnoughSpace then
         r.ffi = t.ffi
       else
-        (s2 = s with <|refs := s.refs
-         |+ ((LEAST ptr. ¬(ptr IN FDOM s.refs)),ByteArray T arr);
-         space := 0;
-         safe_for_space :=
-         (s.safe_for_space /\
-          size_of_heap s + space_consumed (RefByte T) 2 <=
-          s.limits.heap_limit)|> /\
-        arrl = &(LENGTH arr) /\
         ?rv. q = SOME (Result (Loc l1 l2) rv) /\
              state_rel c r1 r2 (s2 with <| locals := LN; clock := new_c |>)
-                r [(RefPtr anyptr,rv)] locs)
+                r [(v,rv)] locs
 Proof
-  fs [RefByteNoInit_code_def]
+  fs [RefByteNoInit_code2_def]
   \\ fs [do_app_def,do_space_def,EVAL ``op_space_reset (RefByte T)``,do_app_aux_def]
   \\ Cases_on `vals` \\ fs []
   \\ Cases_on `t'` \\ fs []
@@ -969,7 +1534,7 @@ Proof
         fs [wordSemTheory.set_var_def,state_rel_insert_1]
   \\ rpt_drule0 AllocVar_thm
    \\ `?x. dataSem$cut_env (fromList [();()]) s.locals = SOME x` by
-    (fs [EVAL ``sptree$fromList [();()]``,cut_env_def,domain_lookup,
+    (fs [EVAL ``sptree$fromList [(); ()]``,cut_env_def,domain_lookup,
          get_var_def,get_vars_SOME_IFF_data])
   \\ disch_then drule0
   \\ fs [wordSemTheory.get_vars_def,wordSemTheory.get_var_def]
@@ -1398,11 +1963,6 @@ Proof
      \\ fs[X_LT_DIV]
   )
   \\ strip_tac \\ fs[]
-  (*continue here *)
-  \\ GEN_EXISTS_TAC"arr"`REPLICATE i w`
-  \\ simp[GSYM PULL_EXISTS] \\ conj_tac
-  >- (simp[allowed_op_def]
-  )
   \\ simp [state_rel_thm]
   \\ fs []
   \\ fs [lookup_def]
@@ -1412,7 +1972,6 @@ Proof
   \\ fs[Abbr`a'`,Abbr`v`,LENGTH_REPLICATE]
   \\ clean_tac
   \\ fs[make_ptr_def,WORD_MUL_LSL]
-  \\ strip_tac \\ qexists_tac`new` \\ pop_assum mp_tac
   \\ qmatch_abbrev_tac`P xx yy zz ⇒ P x' yy z'`
   \\ `xx = x'`
   by (
@@ -1444,6 +2003,167 @@ Proof
   \\ unabbrev_all_tac \\ rpt (pop_assum kall_tac)
   \\ fs[FAPPLY_FUPDATE_THM]
   \\ rw [] \\ fs []
+QED
+
+
+
+(* version with implicit T in immutable
+ * and implicit 0 in initial value
+ *)
+val RefByteNoInit_code3_def = Define `
+  RefByteNoInit_code3 c =
+      let limit = MIN (2 ** c.len_size) (dimword (:'a) DIV 16) in
+      let h = Op Add [Shift Lsr (Var 2) 2; Const bytes_in_word] in
+      let x = SmallLsr h (dimindex (:'a) - 63) in
+      let y = Shift Lsl h (dimindex (:'a) - shift (:'a) - c.len_size) in
+        list_Seq
+          [BignumHalt 2;
+           Assign 1 x;
+           AllocVar c limit (fromList [()]);
+           (* compute length *)
+           Assign 5 (Shift Lsr h (shift (:'a)));
+           Assign 7 (Shift Lsl (Var 5) 2);
+           Assign 9 (Lookup NextFree);
+           (* adjust end of heap *)
+           Assign 1 (Op Add [Var 9;
+                             Shift Lsl (Var 5) (shift (:'a))]);
+           Set NextFree (Op Add [Var 1; Const bytes_in_word]);
+           (* 3 := return value *)
+           Assign 3 (Op Or [Shift Lsl (Op Sub [Var 9; Lookup CurrHeap])
+               (shift_length c − shift (:'a)); Const (1w:'a word)]);
+           (* compute header *)
+           Assign 5 (Op Or [y; Const 7w]);
+           (* store header *)
+           Store (Var 9) 5;
+           (* write last word of byte array *)
+           Assign 11 (Op And [Shift Lsr (Var 2) 2;
+                              Const (bytes_in_word - 1w)]);
+           Assign 13 (Const 0w);
+           Store (Var 1) 13;
+           WriteLastBytes 1 13 11;
+           Assign 7 (Op Sub [Var 7; Const 4w]);
+           (* write rest of byte array *)
+           Call NONE (SOME Replicate_location)
+             (* ret_loc, addr, v, n, ret_val *)
+             [0;9;13;7;3] NONE]:'a wordLang$prog`;
+
+
+Theorem RefByteNoInit_Final_thm:
+   state_rel c l1 l2 s (t:('a,'c,'ffi) wordSem$state) [] locs /\
+    get_vars [0] s.locals = SOME [Number (&arrl)] /\
+    t.clock = MustTerminate_limit (:'a) - 1 /\
+    do_app (RefByte T) ([Number (&arrl)]++[initw]) (dimindex(:'a)) s = Rval (v,s2) ==>
+    ?q r new_c anyptr arr s3.
+     evaluate (RefByteNoInit_code c,t) = (q,r) /\
+      if q = SOME NotEnoughSpace then
+        r.ffi = t.ffi
+      else
+        (s3 = s2 with <|refs := s2.refs
+         |+ ((LEAST ptr. ¬(ptr IN FDOM s.refs)),ByteArray T arr);
+         space := 0;
+         safe_for_space :=
+         (s.safe_for_space /\
+          size_of_heap s + space_consumed (RefByte T) 2 <=
+          s.limits.heap_limit)|> /\
+        arrl = &(LENGTH arr) /\
+        ?rv. q = SOME (Result (Loc l1 l2) rv) /\
+             state_rel c r1 r2 (s3 with <| locals := LN; clock := new_c |>)
+                r [(RefPtr anyptr,rv)] locs)
+Proof
+  cheat (* fs [RefByteNoInit_code_def]
+  \\ fs [do_app_def,do_space_def,EVAL ``op_space_reset (RefByte T)``,do_app_aux_def]
+  \\ Cases_on `initw` \\ fs []
+  \\ IF_CASES_TAC \\ fs [] \\ rw []
+  \\ `good_dimindex (:'a)` by fs [state_rel_def]
+  \\ drule0 NONNEG_INT \\ strip_tac \\ rveq \\ fs []
+  \\ fs[]
+  \\ rename1 `get_vars [0; 1; 2] s.locals = SOME [Number (&i); Word (w2v w); Number &tag]`
+  \\ once_rewrite_tac [list_Seq_def]
+  \\ fs [wordSemTheory.evaluate_def,word_exp_rw]
+  \\ rpt_drule0 state_rel_get_vars_IMP \\ strip_tac \\ fs [LENGTH_EQ_NUM_compute]
+  \\ rveq \\ fs [adjust_var_def,get_vars_SOME_IFF]
+  \\ fs [get_vars_SOME_IFF_data]
+  \\ drule0 (Q.GEN`a1`(Q.SPEC `0` state_rel_get_var_Number_IMP_alt)) \\ fs []
+  \\ strip_tac \\ rveq
+  \\ rpt_drule0 evaluate_BignumHalt
+  \\ Cases_on `small_int (:α) (&i)` \\ fs [] \\ strip_tac \\ fs []
+  \\ ntac 3 (pop_assum kall_tac)
+  \\ once_rewrite_tac [list_Seq_def]
+  \\ fs [wordSemTheory.evaluate_def,word_exp_rw]
+  \\ rpt_drule0 state_rel_get_vars_IMP \\ strip_tac \\ fs [LENGTH_EQ_2]
+  \\ rveq \\ fs [adjust_var_def,get_vars_SOME_IFF]
+  \\ fs [wordSemTheory.get_var_def]
+  \\ `w' = n2w (4 * i) /\ 4 * i < dimword (:'a)` by
+   (fs [state_rel_thm]
+    \\ full_simp_tac std_ss [GSYM APPEND_ASSOC]
+    \\ qpat_x_assum `get_var 0 s.locals = SOME (Number (&i))` assume_tac
+    \\ rpt_drule0 memory_rel_get_var_IMP \\ fs [adjust_var_def]
+    \\ fs [wordSemTheory.get_var_def]
+    \\ strip_tac \\ imp_res_tac memory_rel_Number_IMP
+    \\ fs [Smallnum_def] \\ fs [small_int_def] \\ fs [X_LT_DIV])
+  \\ rveq \\ fs [word_exp_SmallLsr]
+  \\ IF_CASES_TAC
+  THEN1 (fs [shift_def,state_rel_def,
+             EVAL ``good_dimindex (:'a)``] \\ rfs []) \\ fs []
+  \\ pop_assum kall_tac
+  \\ fs [word_exp_rw]
+  \\ IF_CASES_TAC
+  THEN1 (fs [shift_def,state_rel_def,
+             EVAL ``good_dimindex (:'a)``] \\ rfs []) \\ fs []
+  \\ pop_assum kall_tac
+  \\ `n2w (4 * i) ⋙ 2 = (n2w i):'a word` by
+   (rewrite_tac [GSYM w2n_11,w2n_lsr]
+    \\ fs [ONCE_REWRITE_RULE [MULT_COMM] MULT_DIV]) \\ fs []
+  \\ qabbrev_tac `wA = ((bytes_in_word + n2w i)
+        ⋙ (dimindex (:α) − 63)):'a word`
+  \\ once_rewrite_tac [list_Seq_def]
+  \\ fs [wordSemTheory.evaluate_def,word_exp_rw]
+  \\ `state_rel c l1 l2 s (set_var 1 (Word wA) t) [] locs` by
+        fs [wordSemTheory.set_var_def,state_rel_insert_1]
+  \\ rpt_drule0 AllocVar_thm
+   \\ `?x. dataSem$cut_env (fromList [();();()]) s.locals = SOME x` by
+    (fs [EVAL ``sptree$fromList [(); (); ()]``,cut_env_def,domain_lookup,
+         get_var_def,get_vars_SOME_IFF_data])
+  \\ disch_then drule0
+  \\ fs [wordSemTheory.get_vars_def,wordSemTheory.get_var_def]
+  \\ qabbrev_tac `limit = MIN (2 ** c.len_size) (dimword (:α) DIV 16)`
+  \\ fs [get_var_set_var_thm]
+  \\ Cases_on `evaluate
+       (AllocVar c limit (fromList [(); (); ()]),set_var 1 (Word wA) t)` \\ fs []
+  \\ disch_then drule0
+  \\ impl_tac THEN1 (unabbrev_all_tac \\ fs []
+                     \\ fs [state_rel_def,EVAL ``good_dimindex (:'a)``,dimword_def])
+  \\ strip_tac \\ simp[set_vars_sing]
+  \\ IF_CASES_TAC \\ fs[]
+  \\ rveq \\ fs[]
+  \\ fs [dataSemTheory.call_env_def,push_env_def,
+         dataSemTheory.set_var_def,wordSemTheory.set_var_def]
+  \\ qabbrev_tac `new = LEAST ptr. ptr ∉ FDOM s.refs`
+  \\ `new ∉ FDOM s.refs` by metis_tac [LEAST_NOTIN_FDOM]
+  \\ fs [] \\ once_rewrite_tac [list_Seq_def]
+  \\ fs [] \\ once_rewrite_tac [list_Seq_def]
+  \\ fs [] \\ once_rewrite_tac [list_Seq_def]
+  \\ once_rewrite_tac [wordSemTheory.evaluate_def]
+  \\ simp [Once wordSemTheory.evaluate_def]
+  \\ fs [word_exp_rw]
+  \\ `lookup 2 r.locals = SOME (Word (n2w (4 * i)))` by
+   (qabbrev_tac `s9 = s with <|locals := x; space := w2n wA DIV 4 + 1|>`
+    \\ fs [state_rel_def,get_vars_SOME_IFF_data]
+    \\ full_simp_tac std_ss [GSYM APPEND_ASSOC,get_var_def]
+    \\ rpt_drule0 word_ml_inv_get_var_IMP
+    \\ fs [get_var_def,wordSemTheory.get_var_def,adjust_var_def]
+    \\ `lookup 0 s9.locals = SOME (Number (&i))` by
+     (unabbrev_all_tac \\ fs [cut_env_def] \\ rveq
+      \\ fs [lookup_inter_alt] \\ EVAL_TAC)
+    \\ rpt (disch_then drule0) \\ fs []
+    \\ `IS_SOME (lookup 0 s9.locals)` by fs []
+    \\ res_tac \\ Cases_on `lookup 2 r.locals` \\ fs []
+    \\ fs [word_ml_inv_def] \\ rw []
+    \\ fs [abs_ml_inv_def,bc_stack_ref_inv_def,v_inv_def] \\ rfs []
+    \\ rw [] \\ fs [word_addr_def,Smallnum_def]
+    \\ fs [small_int_def,X_LT_DIV]
+    \\ match_mp_tac minus_2_word_and_id
+    \\ fs [word_index,word_mul_n2w,bitTheory.BIT0_ODD,ODD_MULT]) *)
 QED
 
 Theorem RefByte_thm:
